code/bignum/Hacl.Spec.Bignum.Fproduct.fst
@@ -9,7 +9,7 @@ open Hacl.Spec.Bignum.Modulo
 
 module U32 = FStar.UInt32
 
-#set-options "--initial_fuel 1 --max_fuel 1"
+#reset-options "--max_fuel 0 --max_ifuel 0"
 
 let copy_from_wide_pre (s:seqelem_wide) : GTot Type0 =
   (forall (i:nat). {:pattern w (Seq.index s i)} i < len ==> w (Seq.index s i) < pow2 n)
@@ -18,44 +18,28 @@ let copy_from_wide_pre (s:seqelem_wide) : GTot Type0 =
 #set-options "--z3rlimit 20"
 
 val copy_from_wide_spec_: s:seqelem_wide{copy_from_wide_pre s} ->
-  i:nat{i <= len} ->
-  tmp:seqelem{(forall (j:nat). (j >= i /\ j < len) ==> v (Seq.index tmp j) = w (Seq.index s j))} ->
   Tot (s':seqelem{(forall (j:nat). j < len ==> v (Seq.index s' j) = w (Seq.index s j))})
-let rec copy_from_wide_spec_ s i tmp =
-  if i = 0 then tmp
-  else (
-    let i = i - 1 in
-    let si = Seq.index s i in
-    let tmpi = wide_to_limb si in
-    Math.Lemmas.modulo_lemma (w si) (pow2 n);
-    let tmp' = Seq.upd tmp i tmpi in
-    copy_from_wide_spec_ s i tmp'
-  )
+let copy_from_wide_spec_ s =
+  Spec.Loops.seq_map (fun x -> wide_to_limb x) s
 
+#reset-options "--max_fuel 1 --max_ifuel 1 --z3rlimit 50"
 
 val lemma_copy_from_wide_: s:seqelem_wide{copy_from_wide_pre s} -> i:nat{i <= len} ->
-  Lemma (seval_ (copy_from_wide_spec_ s len (Seq.create len limb_zero)) i =
-    seval_wide_ s i)
+  Lemma (seval_ (copy_from_wide_spec_ s) i = seval_wide_ s i)
 let rec lemma_copy_from_wide_ s i =
   if i = 0 then ()
   else lemma_copy_from_wide_ s (i-1)
 
 
-#set-options "--z3rlimit 5"
-
 val copy_from_wide_spec: s:seqelem_wide{copy_from_wide_pre s} ->
   Tot (s':seqelem{(forall (j:nat). j < len ==> v (Seq.index s' j) = w (Seq.index s j))})
-let rec copy_from_wide_spec s =
-  let tmp = Seq.create len limb_zero in
-  copy_from_wide_spec_ s len tmp
+let copy_from_wide_spec s = copy_from_wide_spec_ s
 
 
 val lemma_copy_from_wide: s:seqelem_wide{copy_from_wide_pre s} ->
   Lemma (seval (copy_from_wide_spec s) = seval_wide s)
 let lemma_copy_from_wide s = lemma_copy_from_wide_ s len
 
-
-#set-options "--z3rlimit 5"
 
 val shift_spec: seqelem -> Tot seqelem
 let shift_spec s =
@@ -78,33 +62,28 @@ open FStar.Mul
 let sum_scalar_multiplication_pre_ (sw:seqelem_wide) (s:seqelem) (scalar:limb) (i:nat{i <= len}) : GTot Type0 =
   (forall (j:nat). {:pattern (w (Seq.index sw j)) \/ (v (Seq.index s j))}j < i ==> w (Seq.index sw j) + (v (Seq.index s j) * v scalar) < pow2 wide_n)
 
-#set-options "--z3rlimit 100 --initial_fuel 1 --max_fuel 1"
+private
+val lemma_mod: a:nat -> b:nat -> s:nat -> Lemma
+  (requires (a + b * s < pow2 wide_n))
+  (ensures ((a + b * s) % pow2 wide_n = a + b * s))
+  [SMTPat ((a + b * s) % pow2 wide_n)]
+let lemma_mod a b s =
+  Math.Lemmas.modulo_lemma (a + b * s) (pow2 wide_n)
+
+#reset-options "--z3rlimit 100 --max_fuel 0 --max_ifuel 0"
 
 val sum_scalar_multiplication_spec:
   sw:seqelem_wide ->
   s:seqelem ->
-  scalar:limb ->
-  i:nat{i <= len /\ sum_scalar_multiplication_pre_ sw s scalar i} ->
+  scalar:limb{sum_scalar_multiplication_pre_ sw s scalar len} ->
   Tot (s':seqelem_wide{
-    (forall (j:nat). {:pattern (w (Seq.index s' j))} j < i ==>
-      w (Seq.index s' j) = w (Seq.index sw j) + (v (Seq.index s j) * v scalar))
-    /\ (forall (j:nat). {:pattern (Seq.index s' j)} (j >= i /\ j < len) ==>
-      Seq.index s' j == Seq.index sw j)})
-  (decreases i)
-let rec sum_scalar_multiplication_spec sw s scalar i =
-  if i = 0 then sw
-  else (
-    let j = i - 1 in
-    let swi = Seq.index sw j in
-    let si = Seq.index s j in
-    let open Hacl.Bignum.Wide in
-    let swi' = swi +^ (mul_wide si scalar) in
-    let sw' = Seq.upd sw j swi' in
-    sum_scalar_multiplication_spec sw' s scalar j
-  )
+    (forall (j:nat). {:pattern (w (Seq.index s' j))} j < len ==>
+      w (Seq.index s' j) = w (Seq.index sw j) + (v (Seq.index s j) * v scalar))})
+let sum_scalar_multiplication_spec sw s scalar =
+  Spec.Loops.seq_map2 (fun x y -> Hacl.Bignum.Wide.(x +%^ (y *^ scalar))) sw s
 
 
-#set-options "--max_fuel 0 --initial_fuel 0"
+#reset-options "--max_fuel 0 --max_ifuel 0 --z3rlimit 100"
 
 private val lemma_sum_scalar_multiplication_aux_1: a:nat -> b:nat -> c:nat -> d:nat -> e:nat -> f:nat -> g:nat -> h:nat -> i:nat -> scalar:nat -> v:nat -> Lemma
     (requires (a = v * b + c
@@ -116,16 +95,16 @@ private val lemma_sum_scalar_multiplication_aux_1: a:nat -> b:nat -> c:nat -> d:
 private let lemma_sum_scalar_multiplication_aux_1 a b c d  e f g h i scalar v = ()
 
 
-#set-options "--max_fuel 1 --initial_fuel 1"
+#reset-options "--max_fuel 1 --initial_fuel 1 --z3rlimit 100"
 
 val lemma_sum_scalar_multiplication_:
   sw:seqelem_wide -> s:seqelem -> scalar:limb -> i:nat{i <= len /\ sum_scalar_multiplication_pre_ sw s scalar len} ->
-  Lemma (seval_wide_ (sum_scalar_multiplication_spec sw s scalar len) i = seval_wide_ sw i + (seval_ s i * v scalar))
+  Lemma (seval_wide_ (sum_scalar_multiplication_spec sw s scalar) i = seval_wide_ sw i + (seval_ s i * v scalar))
 let rec lemma_sum_scalar_multiplication_ sw s scalar i =
   if i = 0 then ()
   else (
     lemma_sum_scalar_multiplication_ sw s scalar (i-1);
-    let s' = sum_scalar_multiplication_spec sw s scalar len in
+    let s' = sum_scalar_multiplication_spec sw s scalar in
     cut (w (Seq.index s' (i-1)) = w (Seq.index sw (i-1)) + v (Seq.index s (i-1)) * v scalar);
     cut (seval_wide_ s' i = pow2 (limb_size * (i-1)) * w (Seq.index s' (i-1)) + seval_wide_ s' (i-1));
     cut (seval_wide_ sw i = pow2 (limb_size * (i-1)) * w (Seq.index sw (i-1)) + seval_wide_ sw (i-1));
@@ -134,26 +113,21 @@ let rec lemma_sum_scalar_multiplication_ sw s scalar i =
   )
 
 
-#set-options "--z3rlimit 10"
-
-
 let carry_wide_pre (s:seqelem_wide) (i:nat{i < len}) : GTot Type0 =
   (forall (j:nat). {:pattern (w (Seq.index s j))} (j > i /\ j < len) ==> w (Seq.index s j) < pow2 (wide_n - 1))
   /\ (forall (j:nat). {:pattern (w (Seq.index s j))} (j < i) ==> w (Seq.index s j) < pow2 limb_size)
 
 
-#set-options "--z3rlimit 100 --initial_fuel 1 --max_fuel 1"
-
+#reset-options "--z3rlimit 100 --max_fuel 0 --max_ifuel 0"
 
 val carry_wide_step: s:seqelem_wide ->
-    i:nat{i < len-1 /\ carry_wide_pre s i
-      (* /\ (forall (j:nat). {:pattern (w (Seq.index s j))} j < i ==> w (Seq.index s j) < pow2 limb_size) *)} ->
+    i:nat{i < len-1 /\ carry_wide_pre s i} ->
   Tot (s':seqelem_wide{
     (forall (j:nat). {:pattern (Seq.index s' j)} (j < i \/ (j > i+1 /\ j < len))
                ==> Seq.index s' j == Seq.index s j)
     /\ w (Seq.index s' i) = w (Seq.index s i) % pow2 limb_size
     /\ w (Seq.index s' (i+1)) = w (Seq.index s (i+1)) + (w (Seq.index s i) / pow2 limb_size)
-    (* /\ (forall (j:nat). {:pattern (w (Seq.index s' j))} j < (i+1) ==> w (Seq.index s' j) < pow2 limb_size) *)})
+    })
 let carry_wide_step s i =
     let si = Seq.index s i in
     let sip1 = Seq.index s (i+1) in
@@ -185,7 +159,7 @@ let carry_wide_step s i =
     s''
 
 
-#set-options "--z3rlimit 10 --initial_fuel 2 --max_fuel 2"
+#reset-options "--z3rlimit 100 --initial_fuel 2 --max_fuel 2"
 
 val lemma_carry_wide_step_1: s:seqelem_wide -> i:nat{i < len - 1 /\ carry_wide_pre s i} -> j:nat{j <= i} ->
   Lemma (requires (true))
@@ -193,30 +167,27 @@ val lemma_carry_wide_step_1: s:seqelem_wide -> i:nat{i < len - 1 /\ carry_wide_p
 let rec lemma_carry_wide_step_1 s i j =
   if j = 0 then () else lemma_carry_wide_step_1 s i (j-1)
 
-#set-options "--z3rlimit 100 --initial_fuel 0 --max_fuel 0"
+#reset-options "--z3rlimit 100 --max_fuel 0 --max_ifuel 0"
 
 val lemma_carry_wide_step_2_1: s1':nat -> s0':nat -> s1:nat -> s0:nat -> i:nat -> Lemma
   (requires (s0' = s0 % pow2 limb_size /\ s1' = s1 + s0 / pow2 limb_size))
   (ensures  (pow2 (limb_size * (i+1)) * s1' + pow2 (limb_size * (i)) * s0'
     = pow2 (limb_size * (i+1)) * s1 + pow2 (limb_size * (i)) * s0))
 let lemma_carry_wide_step_2_1 s1' s0' s1 s0 i =
-  Math.Lemmas.lemma_div_mod s1 (pow2 limb_size);
-  cut (s0 + pow2 limb_size * s1 = s0' + pow2 limb_size * s1');
-  cut (pow2 (limb_size * i) * (s0 + pow2 limb_size * s1) = pow2 (limb_size * i) * (s0' + pow2 limb_size * s1'));
-  cut (limb_size * (i+1) = limb_size * i + limb_size);
+  Math.Lemmas.lemma_div_mod s0 (pow2 limb_size);
   Math.Lemmas.pow2_plus (limb_size * i) limb_size;
   Math.Lemmas.distributivity_add_right (pow2 (limb_size * i)) (pow2 limb_size * s1) s0;
   Math.Lemmas.paren_mul_right (pow2 (limb_size * i)) (pow2 limb_size) s1;
   Math.Lemmas.distributivity_add_right (pow2 (limb_size * i)) (pow2 limb_size * s1') s0'
 
 
-#set-options "--z3rlimit 100 --initial_fuel 0 --max_fuel 0"
+#reset-options "--z3rlimit 100 --max_fuel 0 --max_ifuel 0"
 
 val lemma_carry_wide_step_2: s:seqelem_wide -> i:nat{i < len - 1 /\ carry_wide_pre s i
   /\ (forall (j:nat). {:pattern (w (Seq.index s j))} j < i ==> w (Seq.index s j) < pow2 limb_size)} ->
   Lemma (requires (true))
         (ensures (seval_wide_ (carry_wide_step s i) (i+2) = seval_wide_ s (i+2)))
-let rec lemma_carry_wide_step_2 s i =
+let lemma_carry_wide_step_2 s i =
   let s' = carry_wide_step s i in
   lemma_seval_wide_def s' (i+2);
   lemma_seval_wide_def s' (i+1);
@@ -231,6 +202,7 @@ let rec lemma_carry_wide_step_2 s i =
   let s0 = w (Seq.index s (i)) in
   lemma_carry_wide_step_2_1 s1' s0' s1 s0 i;
   lemma_carry_wide_step_1 s i i
+
 
 #set-options "--initial_fuel 1 --max_fuel 1"
 
@@ -248,22 +220,65 @@ val lemma_carry_wide_step: s:seqelem_wide -> i:nat{i < len - 1 /\ carry_wide_pre
 let lemma_carry_wide_step s i = lemma_carry_wide_step_3 s i len
 
 
-#set-options "--z3rlimit 100 --initial_fuel 1 --max_fuel 1"
+#reset-options "--z3rlimit 100 --max_fuel 0 --max_ifuel 0"
 
-val carry_wide_spec: s:seqelem_wide -> i:nat{i < len /\ carry_wide_pre s i} ->
+val carry_wide_step': s:seqelem_wide ->
+    i:nat{i < len-1 /\ carry_wide_pre s i} ->
+  Tot (s':seqelem_wide{carry_wide_pre s' (i+1) /\ seval_wide s' = seval_wide s})
+let carry_wide_step' s i =
+  let s' = carry_wide_step s i in
+  lemma_carry_wide_step s i;
+  Math.Lemmas.lemma_div_lt (w (Seq.index s i)) (2*word_size) limb_size;
+  s'
+
+val carry_wide_spec_: s:seqelem_wide -> i:nat{i < len /\ carry_wide_pre s i} ->
+  k:nat{i <= k /\ k < len} ->
+  Tot (s':seqelem_wide{seval_wide s' = seval_wide s
+    /\ carry_wide_pre s' k
+    /\ (forall (j:nat). {:pattern (w (Seq.index s' j))} (j < k) ==> w (Seq.index s' j) < pow2 limb_size)
+    (* /\ (i < len-1 ==> w (Seq.index s' (len-1)) < w (Seq.index s (len-1)) + pow2 (2*word_size - limb_size)) *)})
+  (decreases (len - 1 - i))
+let rec carry_wide_spec_ s i k =
+  (* Spec.Loops.repeat_range_spec 0 (len-1) carry_wide_step' s *)
+  if i = k then s
+  else (
+    let s'' = carry_wide_step' s i in
+    (* lemma_carry_wide_step s i; *)
+    (* Math.Lemmas.lemma_div_lt (w (Seq.index s i)) (2*word_size) limb_size; *)
+    carry_wide_spec_ s'' (i+1) k
+  )
+
+
+#reset-options "--initial_fuel 2 --max_fuel 2 --z3rlimit 200"
+
+val lemma_carry_wide_spec_:
+  min:nat -> max:nat{min < max /\ max < len} -> s:seqelem_wide{carry_wide_pre s min} -> 
+  Lemma (requires (True))
+        (ensures (
+          (* carry_wide_pre (carry_wide_spec_ s min (max-1))  *)
+          carry_wide_step' (carry_wide_spec_ s min (max-1)) (max-1) == carry_wide_spec_ s min max))
+        (decreases (max - min))
+let rec lemma_carry_wide_spec_ min max x =
+  if min = max - 1 then ()
+  else lemma_carry_wide_spec_ (min+1) max (carry_wide_step' x min)
+
+#reset-options "--initial_fuel 0 --max_fuel 0 --z3rlimit 200"
+
+val carry_wide_spec: s:seqelem_wide{carry_wide_pre s 0} -> (* i:nat{i < len /\ carry_wide_pre s i} -> *)
   Tot (s':seqelem_wide{seval_wide s' = seval_wide s
     /\ (forall (j:nat). {:pattern (w (Seq.index s' j))} (j < len - 1) ==> w (Seq.index s' j) < pow2 limb_size)
     (* /\ (i < len-1 ==> w (Seq.index s' (len-1)) < w (Seq.index s (len-1)) + pow2 (2*word_size - limb_size)) *)})
-  (decreases (len - 1 - i))
-let rec carry_wide_spec s i =
-  if i = len - 1 then s
-  else (
-    let s'' = carry_wide_step s i in
-    lemma_carry_wide_step s i;
-    Math.Lemmas.lemma_div_lt (w (Seq.index s i)) (2*word_size) limb_size;
-    carry_wide_spec s'' (i+1)
-  )
+  (* (decreases (len - 1 - i)) *)
+let (* rec *) carry_wide_spec s =
+  carry_wide_spec_ s 0 (len-1)
 
+  (* if i = len - 1 then s *)
+  (* else ( *)
+  (*   let s'' = carry_wide_step s i in *)
+  (*   lemma_carry_wide_step s i; *)
+  (*   Math.Lemmas.lemma_div_lt (w (Seq.index s i)) (2*word_size) limb_size; *)
+  (*   carry_wide_spec s'' (i+1) *)
+  (* ) *)
 
 
 let carry_limb_pre (s:seqelem) (i:nat{i < len}) : GTot Type0 =
@@ -365,28 +380,53 @@ val lemma_carry_limb_step: s:seqelem -> i:nat{i < len - 1 /\ carry_limb_pre s i}
 let lemma_carry_limb_step s i = lemma_carry_limb_step_3 s i len
 
 
-#set-options "--z3rlimit 100 --initial_fuel 1 --max_fuel 1"
+#reset-options "--z3rlimit 100 --initial_fuel 0 --max_fuel 0"
 
-val carry_limb_spec: s:seqelem -> i:nat{i < len /\ carry_limb_pre s i} ->
-  Tot (s':seqelem{seval s' = seval s})
+val carry_limb_step': s:seqelem ->
+    i:nat{i < len-1 /\ carry_limb_pre s i} ->
+  Tot (s':seqelem{carry_limb_pre s' (i+1) /\ seval s' = seval s})
+let carry_limb_step' s i =
+  let s' = carry_limb_step s i in
+  lemma_carry_limb_step s i;
+  s'
+
+val carry_limb_spec_: s:seqelem -> i:nat{i < len /\ carry_limb_pre s i} -> k:nat{i <= k /\ k < len} ->
+  Tot (s':seqelem{seval s' = seval s /\ carry_limb_pre s' k})
   (decreases (len - 1 - i))
-let rec carry_limb_spec s i =
-  if i = len - 1 then s
+let rec carry_limb_spec_ s i k =
+  if i = k then s
   else (
-    let s'' = carry_limb_step s i in
-    lemma_carry_limb_step s i;
-    carry_limb_spec s'' (i+1)
+    let s'' = carry_limb_step' s i in
+    carry_limb_spec_ s'' (i+1) k
   )
 
 
-#set-options "--z3rlimit 5"
+#reset-options "--initial_fuel 2 --max_fuel 2 --z3rlimit 200"
+
+val lemma_carry_limb_spec_:
+  min:nat -> max:nat{min < max /\ max < len} -> s:seqelem{carry_limb_pre s min} -> 
+  Lemma (requires (True))
+        (ensures (
+          carry_limb_step' (carry_limb_spec_ s min (max-1)) (max-1) == carry_limb_spec_ s min max))
+        (decreases (max - min))
+let rec lemma_carry_limb_spec_ min max x =
+  if min = max - 1 then ()
+  else lemma_carry_limb_spec_ (min+1) max (carry_limb_step' x min)
+
+#reset-options "--initial_fuel 0 --max_fuel 0 --z3rlimit 200"
+
+val carry_limb_spec: s:seqelem{carry_limb_pre s 0} ->
+  Tot (s':seqelem{seval s' = seval s})
+let carry_limb_spec s =
+  carry_limb_spec_ s 0 (len-1)
+
 
 
 let carry_0_to_1_pre (input:seqelem) : GTot Type0 =
   (forall (i:nat). (i > 0 /\ i < len) ==> v (Seq.index input i) < pow2 limb_size)
 
-#set-options "--z3rlimit 50 --initial_fuel 0 --max_fuel 0"
 
+#reset-options "--z3rlimit 50 --initial_fuel 0 --max_fuel 0"
 
 val carry_0_to_1_spec: input:seqelem{carry_0_to_1_pre input} -> Tot (output:seqelem{seval output = seval input
   /\ v (Seq.index output 0) = v (Seq.index input 0) % pow2 limb_size
